Added convergence for ICounter

icounter.fst
@@ -35,7 +35,7 @@ let lemma2 l1 l2 lab lbc lac a b c = ()
 val merge : a:history s o
           -> b:history s o
           -> l:history s o{wellformed l /\ is_lca l a b}
-          -> s
+          -> history s o
 let merge a b l = 
   History.lemma1 l;
   assert (wellformed a);
@@ -46,16 +46,97 @@ let merge a b l =
   lemma1 tr (get_state l);
   assert (get_state a >= get_state l);
 
-  get_state a + get_state b - get_state l
+  (HistLeaf 0 (get_state a + get_state b - get_state l))
+
+assume val axiom1 : a:history s o
+                    -> b:history s o
+                    -> l:history s o{wellformed l /\ is_lca l a b}
+                    -> Lemma (ensures hbeq l (merge a b l))
+
+val isLeaf : h:history s o
+           -> a:history s o
+           -> Tot bool
+let isLeaf h a = 
+hbeq h a &&
+    begin match a with
+    | HistLeaf _ _ -> true
+    | _ -> false
+end
+
+val append_leaf : h:history s o
+                -> l1:list (history s o)
+                -> l2:list (history s o)
+                -> acc:list (history s o)
+                -> Pure (list (history s o))
+                       (requires (forall h'. isLeaf h h' <==> mem h' l1 \/ mem h' l2 \/ mem h' acc))
+                       (ensures (fun l -> forall h'. isLeaf h h' <==> mem h' l))
+let rec append_leaf h l1 l2 acc =
+  match l1, l2 with
+  |[], [] -> acc
+  |x::xs, _ -> append_leaf h xs l2 (x::acc)
+  |[], x::xs -> append_leaf h [] xs (x::acc)
+
+val findleaf : h:history s o
+               -> Tot (l:list (history s o){(forall h'. mem h' l <==> isLeaf h h')})
+let rec findleaf h = 
+  match h with
+  |HistLeaf _ _ -> [h]
+  |HistNode _ _ _ ch1 _ ch2 -> 
+           let l1 = (findleaf ch1) in
+           let l2 = (findleaf ch2) in
+           append_leaf h l1 l2 []
+
+val sum : list (history s o) -> nat
+let rec sum l =
+  match l with
+  |[] -> 0
+  |x::xs -> (get_state x) + (sum xs)
+
+val times : l:nat -> lca:history s o -> nat
+let rec times l lca =
+  match l with
+  |0 -> 0
+  |n -> (get_state lca) + (times (n - 1) lca)
+
+val diff : lca:history s o 
+         -> l:list (history s o)
+         -> a:history s o{mem a l}
+         -> l1:list (history s o) {(forall h'. mem h' l1 ==> mem h' l ) /\ 
+                                  ((sum l1) - (times ((length l1)) lca) - (get_state lca) = 
+                                  ((sum l) - (times (length l) lca) - (get_state a))) /\ (sum l1 = sum l - (get_state a))}
+let rec diff lca l a =
+  match l with
+  |[] -> []
+  |x::xs -> if (x = a) then xs else x::(diff lca xs a)
+
+val mergeall : lca:history s o{wellformed lca} 
+             -> a:history s o {hbeq lca a} 
+             -> l:list (history s o){forall ele. mem ele l ==> hbeq lca ele /\ 
+                                   (forall h' h''. hbeq lca h' /\ hbeq lca h'' ==> is_lca lca h' h'')}
+             -> Tot (res:history s o {(get_state res) = (sum l) + (get_state a) - (times (length l) lca)}) (decreases l)
+let rec mergeall lca a l =
+  match l with
+  |[] -> a
+  |x::xs -> assert (wellformed lca); 
+          assert (is_lca lca a x);
+          axiom1 a x lca;
+          mergeall lca (merge a x lca) xs
+
+val lemma3 : lca:history s o {wellformed lca }
+           -> l:list (history s o){(forall h'. mem h' l ==> hbeq lca h' /\ 
+                                  (forall h' h''. hbeq lca h' /\ hbeq lca h'' ==> is_lca lca h' h''))}
+           -> Lemma (ensures (forall a b. (mem a l /\ mem b l)  ==>
+                            (get_state (mergeall lca a (diff lca l a)) = get_state (mergeall lca b (diff lca l b)))))
+let lemma3 lca l = ()
 
 val commutativity : a:history s o
                   -> b:history s o
                   -> l:history s o{wellformed l /\ is_lca l a b}
-                  -> Lemma (ensures (merge a b l = merge b a l))
+                  -> Lemma (ensures (get_state (merge a b l) = get_state (merge b a l)))
 let commutativity a b l = ()
 
 val idempotence : a:history s o{wellformed a /\ is_lca a a a}
-                -> Lemma (ensures (merge a a a = get_state a))
+                -> Lemma (ensures (get_state (merge a a a) = get_state a))
 let idempotence a = ()
 
 val associativity : h:history s o{wellformed h}
@@ -65,22 +146,32 @@ val associativity : h:history s o{wellformed h}
                 -> lab:history s o{lcau h a b = lab}
                 -> lbc:history s o{lcau h b c = lbc}
                 -> lac:history s o{lcau h c a = lac}
-                -> mab:history s o{hbeq h mab /\ merge_node a b mab /\ get_state mab = merge a b lab}
-                -> mbc:history s o{hbeq h mbc /\ merge_node b c mbc /\ get_state mbc = merge b c lbc}
-                -> m1:history s o{hbeq h m1 /\ merge_node lab lac m1 /\ get_state m1 = merge lab lac (lcau h lab lac) /\ lcau h a mbc = m1}
-                -> m2:history s o{hbeq h m2 /\ merge_node lbc lac m2 /\ get_state m2 = merge lbc lac (lcau h lbc lac) /\ lcau h mab c = m2}
-                -> mabc1: history s o{hbeq h mabc1 /\ merge_node a mbc mabc1 /\ get_state mabc1 = merge a mbc m1}
-                -> mabc2: history s o{hbeq h mabc2 /\ merge_node mab c mabc2 /\ get_state mabc2 = merge mab c m2}
-                -> Lemma (get_state mabc1 = get_state mabc2)
-                
+                -> mab:history s o{hbeq h mab /\ merge_node a b mab /\ get_state mab = get_state (merge a b lab)}
+                -> mbc:history s o{hbeq h mbc /\ merge_node b c mbc /\ get_state mbc = get_state (merge b c lbc)}
+                -> m1:history s o{hbeq h m1 /\ merge_node lab lac m1 /\ get_state m1 = get_state (merge lab lac (lcau h lab lac)) /\ lcau h a mbc = m1}
+                -> m2:history s o{hbeq h m2 /\ merge_node lbc lac m2 /\ get_state m2 = get_state (merge lbc lac (lcau h lbc lac)) /\ lcau h mab c = m2}
+                -> mabc1: history s o{hbeq h mabc1 /\ merge_node a mbc mabc1 /\ get_state mabc1 = get_state (merge a mbc m1)}
+                -> mabc2: history s o{hbeq h mabc2 /\ merge_node mab c mabc2 /\ get_state mabc2 = get_state (merge mab c m2)}
+                -> Lemma (get_state mabc1 = get_state mabc2)               
 let associativity h a b c lab lbc lac mab mbc m1 m2 mabc1 mabc2 = 
   lcau_associative h a b c lab lbc lac;
   let l2 = lcau h lab lac in
   let l1 = lcau h lbc lac in
   lemma2 (get_state l1) (get_state l2) (get_state lab) (get_state lbc) (get_state lac) (get_state a) (get_state b) 
          (get_state c); ()
-  
 
+val convergence : h:history s o{wellformed h}
+                -> lca:history s o{wellformed lca}
+                -> l:list (history s o){(l = findleaf h) /\ (forall h'. mem h' l ==> hbeq lca h') /\ 
+                                       (forall h' h''. hbeq lca h' /\ hbeq lca h'' ==> is_lca lca h' h'')}
+                                       
+                -> Lemma (ensures (forall a b. ((mem a l /\ mem b l)  ==>
+                        (get_state (mergeall lca a (diff lca l a)) = 
+                         get_state (mergeall lca b (diff lca l b))))))                                     
+let convergence h lca l = 
+  lemma3 lca l; 
+  (*)assert (forall a. mem a l ==> is_lca a a a);*) ()
+  
 instance _ : mrdt s o icounter = {
   History.merge = merge;
   History.commutativity = commutativity;
